Split files

src/tools/symbexec/birs_transferLib.sml
@@ -1,0 +1,37 @@
+structure birs_transferLib =
+struct
+
+local
+
+  open HolKernel Parse boolLib bossLib;
+
+
+  (* error handling *)
+  val libname = "bir_symb_transferLib"
+  val ERR = Feedback.mk_HOL_ERR libname
+  val wrap_exn = Feedback.wrap_exn libname
+
+  open birs_stepLib;
+
+open symb_recordTheory;
+open symb_prop_transferTheory;
+open bir_symbTheory;
+
+open bir_symb_sound_coreTheory;
+open HolBACoreSimps;
+open symb_interpretTheory;
+open pred_setTheory;
+
+open bir_exp_substitutionsTheory;
+open birs_composeLib;
+open birs_auxTheory;
+
+val birs_state_ss = rewrites (type_rws ``:birs_state_t``);
+
+in
+
+
+
+end (* local *)
+
+end (* struct *)
