src/tools/symbexec/test-birs_compose.sml
@@ -1,31 +1,12 @@
-structure bir_symb_composeLib =
-struct
 
-local
+open HolKernel Parse boolLib bossLib;
 
-  open HolKernel Parse boolLib bossLib;
+open birs_stepLib;
+open birs_composeLib;
 
-
-  (* error handling *)
-  val libname = "bir_symb_composeLib"
-  val ERR = Feedback.mk_HOL_ERR libname
-  val wrap_exn = Feedback.wrap_exn libname
-
-  open bir_symbLib;
-
-open symb_recordTheory;
-open symb_prop_transferTheory;
-open bir_symbTheory;
-
-open bir_symb_sound_coreTheory;
-open HolBACoreSimps;
-open symb_interpretTheory;
-open pred_setTheory;
-
+open birs_auxTheory;
 
 val birs_state_ss = rewrites (type_rws ``:birs_state_t``);
-
-in
 
 (* testing *)
 val bprog_test_def = Define `
@@ -85,15 +66,6 @@ val birs_rule_STEP_thm =
   (REWRITE_RULE [Once bir_symbTheory.bir_symb_rec_sbir_def]
      (MATCH_MP symb_rulesTheory.symb_rule_STEP_thm birs_symb_step_sound_prog_thm));
 
-val birs_symb_symbst_pc_thm = store_thm(
-   "birs_symb_symbst_pc_thm", ``
-!s.
-  symb_symbst_pc (birs_symb_to_symbst s) = s.bsst_pc
-``,
-  REWRITE_TAC [symb_recordTheory.symb_symbst_pc_def, bir_symbTheory.birs_symb_to_symbst_def]
-);
-
-
 (* first step *)
 val symb_state = ``birs_symb_to_symbst ^birs_state_init``;
 val lbls = ``{^birs_state_init_lbl}``;
@@ -132,84 +104,6 @@ val birs_rule_SEQ_thm =
   (MATCH_MP symb_rulesTheory.symb_rule_SEQ_thm birs_symb_symbols_f_sound_prog_thm);
 
 
-
-val symb_symbols_set_ALT_thm = store_thm(
-   "symb_symbols_set_ALT_thm", ``
-!sr Pi.
-  symb_symbols_set sr Pi = (BIGUNION (IMAGE (symb_symbols sr) Pi))
-``,
-  FULL_SIMP_TAC (std_ss) [symb_symbols_set_def, IMAGE_DEF]
-);
-
-val birs_symb_symbols_set_EQ_thm = store_thm(
-   "birs_symb_symbols_set_EQ_thm", ``
-!prog Pi.
-  symb_symbols_set (bir_symb_rec_sbir prog) (IMAGE birs_symb_to_symbst Pi) = BIGUNION (IMAGE birs_symb_symbols Pi)
-``,
-  FULL_SIMP_TAC (std_ss) [symb_symbols_set_ALT_thm, EXTENSION] >>
-  FULL_SIMP_TAC (std_ss) [IN_BIGUNION_IMAGE] >>
-  FULL_SIMP_TAC (std_ss) [IN_IMAGE] >>
-
-  REPEAT STRIP_TAC >>
-  EQ_TAC >> (
-    REPEAT STRIP_TAC >>
-    FULL_SIMP_TAC (std_ss) [] >>
-    METIS_TAC [bir_symb_sound_coreTheory.birs_symb_symbols_EQ_thm]
-  )
-);
-
-val birs_exps_of_senv_def = Define `
-    birs_exps_of_senv senv =
-      {e | (?vn. senv vn = SOME e)}
-`;
-
-val birs_exps_of_senv_COMP_def = Define `
-    birs_exps_of_senv_COMP excset senv =
-      {e | (?vn. (~(vn IN excset)) /\ senv vn = SOME e)}
-`;
-
-val birs_exps_of_senv_thm = store_thm(
-   "birs_exps_of_senv_thm", ``
-!senv.
-  birs_exps_of_senv senv
-  =
-  birs_exps_of_senv_COMP EMPTY senv
-``,
-  FULL_SIMP_TAC (std_ss++pred_setLib.PRED_SET_ss) [birs_exps_of_senv_COMP_def, birs_exps_of_senv_def]
-);
-
-val birs_exps_of_senv_COMP_thm = store_thm(
-   "birs_exps_of_senv_COMP_thm", ``
-!sr Pi.
-  (!excset. birs_exps_of_senv_COMP excset (K NONE) = EMPTY) /\
-  (!excset senv vn sv. birs_exps_of_senv_COMP excset ((vn =+ (SOME sv)) senv) =
-    if vn IN excset then
-      birs_exps_of_senv_COMP (vn INSERT excset) senv
-    else
-      sv INSERT (birs_exps_of_senv_COMP (vn INSERT excset) senv)) /\
-  (!excset senv vn. birs_exps_of_senv_COMP excset ((vn =+ NONE) senv) = (birs_exps_of_senv_COMP (vn INSERT excset) senv))
-``,
-  REPEAT STRIP_TAC >> (
-    FULL_SIMP_TAC (std_ss++pred_setLib.PRED_SET_ss) [birs_exps_of_senv_COMP_def]
-  ) >>
-
-  Cases_on `vn IN excset` >> (
-    FULL_SIMP_TAC (std_ss++pred_setLib.PRED_SET_ss) [EXTENSION] >>
-    REPEAT STRIP_TAC >> EQ_TAC >> (
-      REPEAT STRIP_TAC >>
-      METIS_TAC [combinTheory.APPLY_UPDATE_THM, optionTheory.option_CLAUSES]
-    )
-  )
-);
-
-val birs_symb_symbols_thm = store_thm(
-   "birs_symb_symbols_thm", ``
-!sys.
-  birs_symb_symbols sys = (BIGUNION (IMAGE bir_vars_of_exp (birs_exps_of_senv sys.bsst_environ))) UNION (bir_vars_of_exp sys.bsst_pcond)
-``,
-  FULL_SIMP_TAC (std_ss) [birs_symb_symbols_def, IMAGE_DEF, birs_exps_of_senv_def, IN_GSPEC_IFF]
-);
-
 val freesymbols_thm = store_thm(
    "freesymbols_thm", ``
 symb_symbols (bir_symb_rec_sbir ^bprog) ^A_sys_tm INTER
@@ -241,9 +135,3 @@ val bprog_composed_thm = save_thm(
 );
 
 (* TODO: tidy up set operations *)
-
-end (* local *)
-
-
-
-end (* struct *)
