src/tools/symbexec/birs_auxScript.sml
@@ -1,0 +1,97 @@
+open HolKernel Parse boolLib bossLib;
+
+open pred_setTheory;
+
+open symb_recordTheory;
+
+open bir_symb_sound_coreTheory;
+
+val _ = new_theory "birs_aux";
+
+val birs_symb_symbst_pc_thm = store_thm(
+   "birs_symb_symbst_pc_thm", ``
+!s.
+  symb_symbst_pc (birs_symb_to_symbst s) = s.bsst_pc
+``,
+  REWRITE_TAC [symb_recordTheory.symb_symbst_pc_def, bir_symbTheory.birs_symb_to_symbst_def]
+);
+
+val symb_symbols_set_ALT_thm = store_thm(
+   "symb_symbols_set_ALT_thm", ``
+!sr Pi.
+  symb_symbols_set sr Pi = (BIGUNION (IMAGE (symb_symbols sr) Pi))
+``,
+  FULL_SIMP_TAC (std_ss) [symb_symbols_set_def, IMAGE_DEF]
+);
+
+val birs_symb_symbols_set_EQ_thm = store_thm(
+   "birs_symb_symbols_set_EQ_thm", ``
+!prog Pi.
+  symb_symbols_set (bir_symb_rec_sbir prog) (IMAGE birs_symb_to_symbst Pi) = BIGUNION (IMAGE birs_symb_symbols Pi)
+``,
+  FULL_SIMP_TAC (std_ss) [symb_symbols_set_ALT_thm, EXTENSION] >>
+  FULL_SIMP_TAC (std_ss) [IN_BIGUNION_IMAGE] >>
+  FULL_SIMP_TAC (std_ss) [IN_IMAGE] >>
+
+  REPEAT STRIP_TAC >>
+  EQ_TAC >> (
+    REPEAT STRIP_TAC >>
+    FULL_SIMP_TAC (std_ss) [] >>
+    METIS_TAC [bir_symb_sound_coreTheory.birs_symb_symbols_EQ_thm]
+  )
+);
+
+val birs_exps_of_senv_def = Define `
+    birs_exps_of_senv senv =
+      {e | (?vn. senv vn = SOME e)}
+`;
+
+val birs_exps_of_senv_COMP_def = Define `
+    birs_exps_of_senv_COMP excset senv =
+      {e | (?vn. (~(vn IN excset)) /\ senv vn = SOME e)}
+`;
+
+val birs_exps_of_senv_thm = store_thm(
+   "birs_exps_of_senv_thm", ``
+!senv.
+  birs_exps_of_senv senv
+  =
+  birs_exps_of_senv_COMP EMPTY senv
+``,
+  FULL_SIMP_TAC (std_ss++pred_setLib.PRED_SET_ss) [birs_exps_of_senv_COMP_def, birs_exps_of_senv_def]
+);
+
+val birs_exps_of_senv_COMP_thm = store_thm(
+   "birs_exps_of_senv_COMP_thm", ``
+!sr Pi.
+  (!excset. birs_exps_of_senv_COMP excset (K NONE) = EMPTY) /\
+  (!excset senv vn sv. birs_exps_of_senv_COMP excset ((vn =+ (SOME sv)) senv) =
+    if vn IN excset then
+      birs_exps_of_senv_COMP (vn INSERT excset) senv
+    else
+      sv INSERT (birs_exps_of_senv_COMP (vn INSERT excset) senv)) /\
+  (!excset senv vn. birs_exps_of_senv_COMP excset ((vn =+ NONE) senv) = (birs_exps_of_senv_COMP (vn INSERT excset) senv))
+``,
+  REPEAT STRIP_TAC >> (
+    FULL_SIMP_TAC (std_ss++pred_setLib.PRED_SET_ss) [birs_exps_of_senv_COMP_def]
+  ) >>
+
+  Cases_on `vn IN excset` >> (
+    FULL_SIMP_TAC (std_ss++pred_setLib.PRED_SET_ss) [EXTENSION] >>
+    REPEAT STRIP_TAC >> EQ_TAC >> (
+      REPEAT STRIP_TAC >>
+      METIS_TAC [combinTheory.APPLY_UPDATE_THM, optionTheory.option_CLAUSES]
+    )
+  )
+);
+
+val birs_symb_symbols_thm = store_thm(
+   "birs_symb_symbols_thm", ``
+!sys.
+  birs_symb_symbols sys = (BIGUNION (IMAGE bir_vars_of_exp (birs_exps_of_senv sys.bsst_environ))) UNION (bir_vars_of_exp sys.bsst_pcond)
+``,
+  FULL_SIMP_TAC (std_ss) [birs_symb_symbols_def, IMAGE_DEF, birs_exps_of_senv_def, IN_GSPEC_IFF]
+);
+
+
+val _ = export_theory();
